Add wait instruction to HTL control path

src/verilog/PrintHTL.ml
@@ -45,7 +45,7 @@ let print_instruction pp (pc, i) =
   fprintf pp "%5d:\t%s" pc (pprint_stmnt 0 i)
 
 let pprint_datapath_stmnt i = function
-  | HTLVstmnt s -> pprint_stmnt i s
+  | HTLDataVstmnt s -> pprint_stmnt i s
   | HTLfork (name, args) -> concat [
       "fork "; extern_atom name; "("; concat (intersperse ", " (List.map register args)); ");\n"
     ]
@@ -55,6 +55,17 @@ let pprint_datapath_stmnt i = function
 
 let print_datapath_instruction pp (pc, i) =
   fprintf pp "%5d:\t%s" pc (pprint_datapath_stmnt 0 i)
+
+let pprint_control_stmnt i = function
+  | HTLCtrlVstmnt s -> pprint_stmnt i s
+  | HTLwait (name, statereg, expr) -> concat [
+      "wait("; extern_atom name; ", ";
+      register statereg; ", ";
+      pprint_expr expr; ");\n"
+    ]
+
+let print_control_instruction pp (pc, i) =
+  fprintf pp "%5d:\t%s" pc (pprint_control_stmnt 0 i)
 
 let ptree_to_list ptree =
   List.sort
@@ -70,7 +81,7 @@ let print_module pp id f =
   fprintf pp "datapath {\n";
   List.iter (print_datapath_instruction pp) datapath;
   fprintf pp "  }\n\n  controllogic {\n";
-  List.iter (print_instruction pp) controllogic;
+  List.iter (print_control_instruction pp) controllogic;
   fprintf pp "  }\n}\n\n"
 
 let print_globdef pp (id, gd) =
